polygen/LoopUnroll.v
@@ -1,4 +1,5 @@
 Require Import List.
+Require Import Lia.
 Require Import ZArith.
 Import ListNotations.
 
@@ -12,6 +13,22 @@ Module Instr := PolIRs.Instr.
 Module State := PolIRs.State.
 Module Loop := PolIRs.Loop.
 Module Subst := LoopSingletonCleanup PolIRs.
+
+Definition succ_expr (e: Loop.expr) : Loop.expr :=
+  Loop.Sum e (Loop.Constant 1).
+
+Fixpoint peel_unroll_stmt_list
+    (fuel: nat) (cur ub: Loop.expr) (body: Loop.stmt) : Loop.stmt_list :=
+  match fuel with
+  | O =>
+      Loop.SCons (Loop.Loop cur ub body) Loop.SNil
+  | S fuel' =>
+      Loop.SCons
+        (Loop.Guard
+           (Loop.LE (succ_expr cur) ub)
+           (Subst.subst_stmt_at 0 cur body))
+        (peel_unroll_stmt_list fuel' (succ_expr cur) ub body)
+  end.
 
 Fixpoint seq_values (vals: list Z) (body: Loop.stmt) : Loop.stmt_list :=
   match vals with
@@ -55,6 +72,128 @@ Proof.
       end.
 Qed.
 
+Lemma seq_single_loop_semantics :
+  forall cur ub body env mem1 mem2,
+    Loop.loop_semantics
+      (Loop.Seq (Loop.SCons (Loop.Loop cur ub body) Loop.SNil))
+      env mem1 mem2 <->
+    Loop.loop_semantics (Loop.Loop cur ub body) env mem1 mem2.
+Proof.
+  intros cur ub body env mem1 mem2.
+  split; intros Hsem.
+  - inversion_clear Hsem.
+    inversion H0; subst; clear H0.
+    exact H.
+  - eapply Loop.LSeq.
+    + exact Hsem.
+    + constructor.
+Qed.
+
+Lemma peel_unroll_stmt_list_semantics :
+  forall fuel cur ub body env mem1 mem2,
+    Loop.loop_semantics
+      (Loop.Seq (peel_unroll_stmt_list fuel cur ub body))
+      env mem1 mem2 <->
+    Loop.loop_semantics (Loop.Loop cur ub body) env mem1 mem2.
+Proof.
+  induction fuel as [|fuel IH]; intros cur ub body env mem1 mem2; simpl.
+  - apply seq_single_loop_semantics.
+  - remember (Loop.eval_expr env cur) as curv.
+    remember (Loop.eval_expr env ub) as ubv.
+    assert (Htest_true :
+      Loop.eval_test env (Loop.LE (succ_expr cur) ub) = true <->
+      curv < ubv).
+    {
+      subst curv ubv. simpl. rewrite Z.leb_le. lia.
+    }
+    assert (Htest_false :
+      Loop.eval_test env (Loop.LE (succ_expr cur) ub) = false <->
+      curv >= ubv).
+    {
+      subst curv ubv. simpl. rewrite Z.leb_gt. lia.
+    }
+    split; intros Hsem.
+    + inversion_clear Hsem.
+      apply IH in H0.
+      destruct (Z_lt_ge_dec curv ubv) as [Hlt|Hge].
+      * apply Loop.LLoop.
+        rewrite <- Heqcurv, <- Hequbv.
+        rewrite Zrange_begin by lia.
+        inversion H; subst; clear H.
+        -- match goal with
+           | Hbody: Loop.loop_semantics (Subst.subst_stmt_at 0 cur body) env _ _,
+             Hguard: Loop.eval_test env (Loop.LE (succ_expr cur) ub) = true |- _ =>
+               apply Subst.subst_stmt_at_semantics in Hbody;
+               simpl in Hbody;
+               inversion_clear H0;
+               econstructor; eauto
+           end.
+        -- match goal with
+           | Hguard: Loop.eval_test env (Loop.LE (succ_expr cur) ub) = false |- _ =>
+               apply Htest_false in Hguard; lia
+           end.
+      * inversion H; subst; clear H.
+        -- match goal with
+           | Hguard: Loop.eval_test env (Loop.LE (succ_expr cur) ub) = true |- _ =>
+               apply Htest_true in Hguard; lia
+           end.
+        -- inversion H0; subst; clear H0.
+           match goal with
+           | Hiter: _ |- _ =>
+               simpl in Hiter;
+               rewrite Zrange_empty in Hiter by lia;
+               inversion Hiter; subst
+           end.
+           apply Loop.LLoop.
+           simpl.
+           rewrite Zrange_empty by lia.
+           constructor.
+    + inversion_clear Hsem.
+      destruct (Z_lt_ge_dec curv ubv) as [Hlt|Hge].
+      * match goal with
+        | Hiter: PolIRs.Instr.IterSem.iter_semantics
+            (fun x : Z => Loop.loop_semantics body (x :: env))
+            (Zrange _ _) _ _ |- _ =>
+            rewrite <- Heqcurv, <- Hequbv in Hiter;
+            rewrite Zrange_begin in Hiter by lia;
+            inversion_clear Hiter
+        end.
+        eapply Loop.LSeq.
+        -- apply Loop.LGuardTrue.
+           ++ apply Subst.subst_stmt_at_semantics.
+              simpl.
+              rewrite <- Heqcurv.
+              match goal with
+              | Hbody: Loop.loop_semantics body (curv :: env) _ _ |- _ =>
+                  exact Hbody
+              end.
+           ++ apply Htest_true. exact Hlt.
+        -- apply IH.
+           apply Loop.LLoop.
+           simpl.
+           rewrite <- Heqcurv, <- Hequbv.
+           match goal with
+           | Htail: Instr.IterSem.iter_semantics _ (Zrange (curv + 1) ubv) _ _ |- _ =>
+               exact Htail
+           end.
+      * match goal with
+        | Hiter: PolIRs.Instr.IterSem.iter_semantics
+            (fun x : Z => Loop.loop_semantics body (x :: env))
+            (Zrange _ _) _ _ |- _ =>
+            rewrite <- Heqcurv, <- Hequbv in Hiter;
+            rewrite Zrange_empty in Hiter by lia;
+            inversion Hiter; subst; clear Hiter
+        end.
+        eapply Loop.LSeq.
+        -- apply Loop.LGuardFalse.
+           apply Htest_false. exact Hge.
+        -- apply IH.
+           apply Loop.LLoop.
+           simpl.
+           rewrite Zrange_empty by lia.
+           constructor.
+Qed.
+
 Fixpoint const_unroll_stmt (st: Loop.stmt) : Loop.stmt :=
   match st with
   | Loop.Loop (Loop.Constant lb) (Loop.Constant ub) body =>
@@ -85,6 +224,39 @@ with const_unroll_stmt_list_changed (sts: Loop.stmt_list) : bool :=
   | Loop.SNil => false
   | Loop.SCons st sts' =>
       orb (const_unroll_stmt_changed st) (const_unroll_stmt_list_changed sts')
+  end.
+
+Fixpoint peel_unroll_stmt (fuel: nat) (st: Loop.stmt) : Loop.stmt :=
+  match st with
+  | Loop.Loop lb ub body =>
+      Loop.Seq (peel_unroll_stmt_list fuel lb ub body)
+  | Loop.Instr i es => Loop.Instr i es
+  | Loop.Seq sts => Loop.Seq (peel_unroll_stmt_list_rec fuel sts)
+  | Loop.Guard t body => Loop.Guard t (peel_unroll_stmt fuel body)
+  end
+with peel_unroll_stmt_list_rec (fuel: nat) (sts: Loop.stmt_list) : Loop.stmt_list :=
+  match sts with
+  | Loop.SNil => Loop.SNil
+  | Loop.SCons st sts' =>
+      Loop.SCons (peel_unroll_stmt fuel st) (peel_unroll_stmt_list_rec fuel sts')
+  end.
+
+Fixpoint peel_unroll_stmt_changed (fuel: nat) (st: Loop.stmt) : bool :=
+  match fuel with
+  | O => false
+  | S _ =>
+      match st with
+      | Loop.Loop _ _ _ => true
+      | Loop.Instr _ _ => false
+      | Loop.Seq sts => peel_unroll_stmt_list_changed fuel sts
+      | Loop.Guard _ body => peel_unroll_stmt_changed fuel body
+      end
+  end
+with peel_unroll_stmt_list_changed (fuel: nat) (sts: Loop.stmt_list) : bool :=
+  match sts with
+  | Loop.SNil => false
+  | Loop.SCons st sts' =>
+      orb (peel_unroll_stmt_changed fuel st) (peel_unroll_stmt_list_changed fuel sts')
   end.
 
 Scheme stmt_ind_mut := Induction for Loop.stmt Sort Prop
@@ -144,6 +316,46 @@ Proof.
     + apply <- H in H1. apply <- H0 in H2. econstructor; eauto.
 Qed.
 
+Theorem peel_unroll_stmt_correct :
+  forall fuel,
+  (forall st env mem1 mem2,
+      Loop.loop_semantics (peel_unroll_stmt fuel st) env mem1 mem2 <->
+      Loop.loop_semantics st env mem1 mem2)
+  /\
+  (forall sts env mem1 mem2,
+      Loop.loop_semantics (Loop.Seq (peel_unroll_stmt_list_rec fuel sts)) env mem1 mem2 <->
+      Loop.loop_semantics (Loop.Seq sts) env mem1 mem2).
+Proof.
+  intro fuel.
+  apply stmt_stmt_list_ind; intros; simpl.
+  - split; intros Hsem.
+    + apply peel_unroll_stmt_list_semantics in Hsem.
+      exact Hsem.
+    + inversion_clear Hsem.
+      apply peel_unroll_stmt_list_semantics.
+      apply Loop.LLoop.
+      exact H0.
+  - split; intros Hsem; exact Hsem.
+  - split; intros Hsem.
+    + apply H. exact Hsem.
+    + apply <- H. exact Hsem.
+  - split; intros Hsem; inversion_clear Hsem as [| | | ? ? ? ? ? Hbody Heq | ? ? ? ? Heq |].
+    + apply Loop.LGuardTrue; [apply H; exact Hbody|exact Heq].
+    + apply Loop.LGuardFalse. exact Heq.
+    + apply Loop.LGuardTrue; [apply <- H; exact Hbody|exact Heq].
+    + apply Loop.LGuardFalse. exact Heq.
+  - split; intros Hsem; inversion_clear Hsem; constructor.
+  - split; intros Hsem; inversion_clear Hsem.
+    + apply H in H1. apply H0 in H2. econstructor; eauto.
+    + apply <- H in H1. apply <- H0 in H2. econstructor; eauto.
+Qed.
+
+Lemma peel_unroll_stmt_semantics :
+  forall fuel st env mem1 mem2,
+    Loop.loop_semantics (peel_unroll_stmt fuel st) env mem1 mem2 <->
+    Loop.loop_semantics st env mem1 mem2.
+Proof. intros. apply peel_unroll_stmt_correct. Qed.
+
 Lemma const_unroll_stmt_semantics :
   forall st env mem1 mem2,
     Loop.loop_semantics (const_unroll_stmt st) env mem1 mem2 <->
@@ -157,6 +369,14 @@ Definition const_unroll (prog: Loop.t) : Loop.t :=
 Definition const_unroll_changed (prog: Loop.t) : bool :=
   let '(st, _, _) := prog in
   const_unroll_stmt_changed st.
+
+Definition peel_unroll (fuel: nat) (prog: Loop.t) : Loop.t :=
+  let '(st, ctxt, vars) := prog in
+  (peel_unroll_stmt fuel st, ctxt, vars).
+
+Definition peel_unroll_changed (fuel: nat) (prog: Loop.t) : bool :=
+  let '(st, _, _) := prog in
+  peel_unroll_stmt_changed fuel st.
 
 Theorem const_unroll_correct :
   forall prog mem1 mem2,
@@ -180,6 +400,30 @@ Proof.
     + exact H1.
     + exact H2.
     + eapply const_unroll_stmt_semantics. exact H3.
+Qed.
+
+Theorem peel_unroll_correct :
+  forall fuel prog mem1 mem2,
+    Loop.semantics (peel_unroll fuel prog) mem1 mem2 <->
+    Loop.semantics prog mem1 mem2.
+Proof.
+  intros fuel prog mem1 mem2.
+  destruct prog as [[st ctxt] vars]; simpl.
+  split; intros Hsem; inversion_clear Hsem; subst.
+  - inversion H; subst.
+    econstructor.
+    + reflexivity.
+    + exact H0.
+    + exact H1.
+    + exact H2.
+    + eapply peel_unroll_stmt_semantics. exact H3.
+  - inversion H; subst.
+    econstructor.
+    + reflexivity.
+    + exact H0.
+    + exact H1.
+    + exact H2.
+    + eapply peel_unroll_stmt_semantics. exact H3.
 Qed.
 
 End LoopUnroll.
