syntax/SLoopUnroll.v
@@ -8,3 +8,9 @@ Definition const_unroll : SPolIRs.Loop.t -> SPolIRs.Loop.t :=
 
 Definition const_unroll_changed : SPolIRs.Loop.t -> bool :=
   CoreUnroll.const_unroll_changed.
+
+Definition peel_unroll : nat -> SPolIRs.Loop.t -> SPolIRs.Loop.t :=
+  CoreUnroll.peel_unroll.
+
+Definition peel_unroll_changed : nat -> SPolIRs.Loop.t -> bool :=
+  CoreUnroll.peel_unroll_changed.
